rustfrontend/RustIRspec.v
@@ -1,0 +1,749 @@
+Require Import Coqlib.
+Require Import Errors.
+Require Import Maps.
+Require Import Integers.
+Require Import Floats.
+Require Import Values.
+Require Import AST Errors.
+Require Import Events.
+Require Import Globalenvs.
+Require Import Smallstep SmallstepSafe.
+Require Import Listmisc.
+Require Import Cop RustOp.
+Require Import Ctypes Rusttypes Rustlight.
+Require Import RustIR.
+Require Import LanguageInterface.
+
+Import ListNotations.
+
+Local Open Scope error_monad_scope.
+
+(** RustIR functional specification. *)
+
+(* Function environment *)
+
+(* Structured values. The structure is similar to the type of this
+value. *)
+Inductive sval : Type :=
+| sv_bot
+| sv_scalar (v: val)            (* scalar value: v cannot be Vptr *)
+| sv_box (sv: sval) 
+| sv_struct (id: ident) (svl: list (ident * sval))
+| sv_enum (id: ident) (fid: ident) (sv: sval)
+| sv_ref (ph: path) (* reference to an owner at [phs] *)
+.
+
+Definition sv_map := PTree.t sval.
+
+(* Operations for sval *)
+
+Definition sem_cast (sv : sval) (t1 t2 : type) : res sval :=
+  match sv with
+  | sv_scalar v =>
+      match sem_cast v t1 t2 with
+      | Some v1 => OK (sv_scalar v1)
+      | None => Error nil
+      end
+  (* We do not support casting for other kinds of value for now *)
+  | _ => OK sv
+  end.
+
+Definition val_casted (sv: sval) (ty: type) : Prop :=
+  match sv with
+  | sv_scalar v =>
+      val_casted v ty
+  | _ => True
+  end.
+
+
+Inductive val_casted_list : list sval -> typelist -> Prop :=
+  | vcl_nil : val_casted_list nil Tnil
+  | vcl_cons : forall (v1 : sval) (vl : list sval) (ty1 : type) (tyl : typelist),
+               val_casted v1 ty1 ->
+               val_casted_list vl tyl -> val_casted_list (v1 :: vl) (Tcons ty1 tyl).
+
+(* Operations for the environment *)
+
+Fixpoint get_owner_sval (phl: list projection) (sv: sval) : res sval :=
+  match phl with
+  | nil => OK sv
+  | ph :: l =>
+      match ph, sv with
+      | proj_deref, sv_box sv1 =>
+          get_owner_sval l sv1
+      | proj_field fid, sv_struct _ fpl =>
+          match find_field fid fpl with
+          | Some sv1 =>
+              get_owner_sval l sv1
+          | None => Error nil
+          end
+      | proj_downcast fid1, sv_enum _ fid2 sv1 =>
+          if ident_eq fid1 fid2 then
+            get_owner_sval l sv1
+          else
+            Error nil
+      | _, _  => Error nil
+      end
+  end.
+
+Definition get_owner_sval_map (ph: path) (e: sv_map) : res sval :=
+  let (id, pj) := ph in
+  match e ! id with
+  | Some sv =>
+      get_owner_sval pj sv
+  | None =>
+      Error nil
+  end.
+
+(* To get the location of arbitary path, we divide it into two steps:
+first we use [get_owner_path] to obtain the path of these projections
+in the tree and second we use [get_owner_sval] to obtain its sval. *)
+Fixpoint get_owner_path (e: sv_map) (ph: path) (phl: list projection) (sv: sval)  : res path :=
+  match phl with
+  | nil => OK ph
+  | pj :: l =>
+      let ph1 := (fst ph, snd ph ++ [pj]) in
+      match pj, sv with
+      | proj_deref, sv_box sv1 =>
+          get_owner_path e ph1 l sv1
+      | proj_field fid, sv_struct _ fpl =>
+          match find_field fid fpl with
+          | Some sv1 =>
+              get_owner_path e ph1 l sv1
+          | None => Error nil
+          end
+      | proj_downcast _, sv_enum _ _ sv1 =>
+          get_owner_path e ph1 l sv1
+      | proj_deref, sv_ref ph2 =>
+          do fp2 <- get_owner_sval_map ph2 e;
+          get_owner_path e ph2 l fp2
+      | _, _  => Error nil
+      end
+  end.
+
+(* This actually can be used to define "reachability" *)
+Definition get_owner_path_sv_map (ps: path) (e: sv_map) : res path :=
+  let (id, phl) := ps in
+  match e!id with
+  | Some sv =>
+      get_owner_path e (id, nil) phl sv
+  | _ => Error nil
+  end.
+
+
+Definition set_field_sv (fid: ident) (v: sval) (svl: list (ident * sval)) : list (ident * sval) :=
+  set_field fid (fun _ => v) svl.
+
+Fixpoint set_sval (phl: list projection) (v: sval) (root: sval) : res sval :=
+  match phl with
+  | nil => OK v
+  | ph :: l =>
+      match ph, root with
+      | proj_deref, sv_box sv1 =>
+          do sv2 <- set_sval l v sv1;
+          OK (sv_box sv2)
+      | proj_field fid, sv_struct id svl =>
+          match find_field fid svl with
+          | Some fsv =>
+              do fsv1 <- set_sval l v fsv;
+              OK (sv_struct id (set_field_sv fid fsv1 svl)) 
+          | None => Error nil
+          end
+      | proj_downcast fid, sv_enum id fid1 sv1 =>
+          if ident_eq fid fid1 then
+            do sv2 <- set_sval l v sv1;
+            OK (sv_enum id fid1 sv2)
+          else Error nil
+      | _, _ => Error nil
+      end
+  end.
+
+Definition set_sval_map (ph: path) (v: sval) (e: sv_map) : res sv_map :=
+  let (id, phl) := ph in
+  match e!id with
+  | Some sv =>
+      do sv1 <- set_sval phl v sv;
+      OK (PTree.set id sv1 e)
+  | None => Error nil
+  end.
+
+
+Fixpoint clear_sval_rec (fp: sval) : sval :=
+  match fp with
+  | sv_scalar _
+  (* What about moving a reference? *)
+  | sv_ref _
+  | sv_bot => fp
+  | sv_box fp1 => sv_box sv_bot
+  | sv_enum id fid ffp => sv_enum id fid (clear_sval_rec ffp)
+  | sv_struct id fpl =>
+      sv_struct id (map (fun '(fid, sv) => (fid, clear_sval_rec sv)) fpl)
+  end.
+
+Definition clear_sval_map (ph: path) (e: sv_map) : res sv_map :=
+  do sv <- get_owner_sval_map ph e;
+  set_sval_map ph (clear_sval_rec sv) e.
+
+(* Operations for the function call and return *)
+
+(** Some generic operations for adding and collecting paths from fpm or sv_map *)
+
+Definition add_ref_path (ph: path) (l: list path) : list path :=
+  if existsb (fun ph1 => is_prefix_path ph1 ph) l then
+    l
+  else
+    (* We keep the non-prefix paths *)
+    let l1 := filter (fun ph1 => negb (is_prefix_path ph ph1)) l in
+    ph :: l.
+
+Fixpoint add_ref_paths (l acc: list path) : list path :=
+  match l with
+  | nil => acc
+  | ph :: l' =>
+      add_ref_paths l' (add_ref_path ph acc)
+  end.
+
+Definition lex_ord_lt := lex_ord lt lt.
+
+Lemma remove_first_length_lt {A B: Type} eqA : forall (l1: list A) (l2 l2': list B) x 
+    (InH: In x l1),
+    lex_ord_lt (length (remove eqA x l1), length l2)  (length l1, length l2').
+Proof.
+  intros. eapply lex_ord_left.
+  eapply remove_length_lt. auto.
+Qed.
+
+Lemma lex_lt_cons_snd {A B: Type} : forall (l1: list A) (l2 l2': list B) x
+    (EQ: l2' = x :: l2),
+    lex_ord_lt (length l1, length l2)  (length l1, length l2').
+Proof.
+  intros. rewrite EQ.
+  eapply lex_ord_right. simpl. 
+  econstructor.
+Qed.
+
+(* Recursively collect ref paths. The actual definition of get_paths
+depends on the definition of structured memory *)
+Fixpoint collect_ref_paths_generic (get_paths: path -> res (list path)) (collected: list path) (to_visit: list path) (not_visited: list path) (ACC: Acc lex_ord_lt (length not_visited, length to_visit)) {struct ACC} : res (list path) :=
+  (match to_visit as to_visit0 return (to_visit = to_visit0) -> res (list path) with
+  | nil => fun _ => OK collected
+  | ph :: to_visit1 =>
+      fun eqH =>
+        match in_dec path_eq ph not_visited with
+        | left InH =>
+            let not_visited1 := (remove path_eq ph not_visited) in
+            let collected1 := add_ref_path ph collected in
+            do new_paths <- get_paths ph;
+            let ACC1 := Acc_inv ACC (remove_first_length_lt path_eq not_visited (new_paths ++ to_visit1) to_visit ph InH) in
+            collect_ref_paths_generic get_paths collected1 (new_paths ++ to_visit1) not_visited1 ACC1
+        (* This ph has been visited so we skip it *)
+        | right _ =>
+            let ACC1 := Acc_inv ACC (lex_lt_cons_snd not_visited to_visit1 to_visit ph eqH) in
+            collect_ref_paths_generic get_paths collected to_visit1 not_visited ACC1
+        end
+  end) eq_refl.
+
+Lemma lex_ord_lt_acc_intro {A B: Type} : forall (l1: list A) (l2: list B),
+    Acc lex_ord_lt (length l1, length l2).
+Proof. 
+  intros.
+  eapply wf_lex_ord. all: eapply Nat.lt_wf_0.
+Qed.
+
+Definition suffix_projections (phl1 phl2: list projection) : list projection :=
+  skipn (length phl1) phl2.
+
+(* We do not return (option path) to simplify the semantics. Note that
+our final goal is to prove no UB in this semantics, so we need to
+ensure that None case is impossible *)
+Definition generate_new_suffix_path (l: list path) (ph: path) : res path :=
+  match list_find (fun ph1 => is_prefix_path ph1 ph) l with
+  | Some (idx, ph1) =>
+      (* We cannot convert zero *)
+      let new_id := Pos.of_nat (S idx) in
+      let pj := suffix_projections (snd ph1) (snd ph) in
+      OK (new_id, pj)
+  | None => Error nil
+  end.
+
+(* The reverse operaiton of generate_new_suffix_path *)
+(* ph= (id, pj) is the returned path where id can be seen as the index
+of the l *)
+Definition recover_ref_path (l: list path) (ph: path) : res path :=
+  let (id, pj) := ph in
+  match nth_error l (pred (Pos.to_nat id)) with
+  | Some ph1 =>
+      (* ph1 is the path in the caller's svm, the actual path of ph
+      should be defined as appending the projecitons of ph into the
+      projetions of ph1 *)
+      OK ((fst ph1, snd ph1 ++ pj))
+  | None =>
+      Error nil
+  end.
+
+
+(** Implementation dependent operations *)
+
+(* collect the owner paths stored in the leaf nodes that are sv_ref *)
+Fixpoint collect_sval_ref_paths (sv: sval) : list path :=
+  match sv with
+  | sv_struct _ svl =>
+      flat_map  (fun '(_, fsv) => collect_sval_ref_paths fsv) svl
+  | sv_enum _ _ fsv =>
+      collect_sval_ref_paths fsv
+  | sv_box sv1 =>
+      collect_sval_ref_paths sv1
+  | sv_ref ph =>
+      ph :: nil
+  | _ => nil
+  end.
+
+Definition collect_svm_ref_paths (svm: sv_map) : list path :=
+  let svl := map (fun '(_, sv) => sv) (PTree.elements svm) in
+  flat_map collect_sval_ref_paths svl.
+
+Definition get_owner_sval_map_ref_paths (svm: sv_map) (ph: path) : res (list path) :=
+  do sv <- get_owner_sval_map ph svm;
+  OK (collect_sval_ref_paths sv).
+
+(* We need to ensure that all the returned paths are disjoint, its
+located note contain deep_init sval, and form a closure *)
+Definition collect_svm_args_ref_paths (svm: sv_map) (args: list sval) : res (list path) :=
+  let not_visited := collect_svm_ref_paths svm in
+  let to_visit := flat_map collect_sval_ref_paths args in
+  collect_ref_paths_generic (get_owner_sval_map_ref_paths svm) nil to_visit not_visited (lex_ord_lt_acc_intro _ _).
+
+
+Fixpoint generate_new_suffix_path_sval (l: list path) (sv: sval) : res sval :=
+  match sv with
+  | sv_ref ph =>
+      do ph1 <- generate_new_suffix_path l ph;
+      OK (sv_ref ph1)
+  | sv_box sv1 =>
+      do sv1' <- generate_new_suffix_path_sval l sv1;
+      OK (sv_box sv1')
+  | sv_struct id svl =>
+      do svl1 <- (mmap (fun '(fid, fsv) => 
+                            do fsv1 <- generate_new_suffix_path_sval l fsv;
+                            OK (fid, fsv1)) svl);
+      OK (sv_struct id svl1)
+  | sv_enum id fid fsv =>
+      do fsv1 <- generate_new_suffix_path_sval l fsv;
+      OK (sv_enum id fid fsv1)
+  | _ => OK sv
+  end.
+
+(* Collect the svals that are passed via reference to the environment *)
+Definition collect_svm_passed_ref_sval (svm: sv_map) (l: list path) : res (list sval) :=
+  mmap (fun ph => do sv <- get_owner_sval_map ph svm;
+               generate_new_suffix_path_sval l sv) l.
+
+(* set sv_bot to the location that passed via reference *)
+Fixpoint clear_svm_passed_ref_sval (svm: sv_map) (l: list path) : res sv_map :=
+  match l with
+  | nil => OK svm
+  | ph :: phl =>
+      do svm1 <- set_sval_map ph sv_bot svm;
+      clear_svm_passed_ref_sval svm1 phl
+  end.
+
+(* The output parameters contain two parts: one for the normal
+arguments and the others are the memory locations passed via
+reference *)
+Definition generate_output_parameters (svm: sv_map) (args: list sval) : res (list sval * list sval * list path) :=
+  do extern_paths <- collect_svm_args_ref_paths svm args;
+  do args1 <- mmap (generate_new_suffix_path_sval extern_paths) args;
+  do extern_svs <- collect_svm_passed_ref_sval svm extern_paths;
+  OK (args1, extern_svs, extern_paths).
+
+Fixpoint recover_sval_ref_paths (l: list path) (sv: sval)  : res sval :=
+  match sv with
+  | sv_ref ph =>
+      do ph1 <- recover_ref_path l ph;
+      OK (sv_ref ph1)
+  | sv_box sv1 =>
+      do sv1' <- recover_sval_ref_paths l sv1;
+      OK (sv_box sv1')
+  | sv_struct id svl =>
+      do svl1 <- mmap (fun '(fid, fsv) => 
+                        do fsv1 <- recover_sval_ref_paths l fsv;
+                        OK (fid, fsv1)) svl;
+      OK (sv_struct id svl1)
+  | sv_enum id fid fsv =>
+      do fsv1 <- recover_sval_ref_paths l fsv;
+      OK (sv_enum id fid fsv1)
+  | _ =>
+      OK sv
+  end.
+
+
+(* When the caller receives the returned sval and the
+reference-passed sval list, it updates their reference paths and
+then putback to the svm. The caller should guarantee that the external
+svals are normalized into the form same as those passed by the
+caller *)
+Definition receive_return_sval (svm: sv_map) (l: list path) (retv: sval) (externs: list sval) : res (sval * sv_map) :=
+  do retv1 <- recover_sval_ref_paths l retv;
+  do externs1 <- mmap (recover_sval_ref_paths l) externs;
+  let phs_externs := combine l externs1 in
+  do svm1 <- mfold_left (fun acc '(ph, sv) => set_sval_map ph sv acc) phs_externs svm;
+  OK (retv1, svm1).
+
+Section SEMANTICS.
+
+(** ** Global environment  *)
+
+Definition rustir_defmap := PTree.t (globdef fundef type).
+
+Record genv := { genv_genv:> Genv.t fundef type; genv_defmap :> rustir_defmap ; genv_cenv :> composite_env; genv_dropm :> PTree.t ident }.
+  
+Definition globalenv (se: Genv.symtbl) (p: program) :=
+  {| genv_genv:= Genv.globalenv se p; genv_defmap := prog_defmap p ; genv_cenv := p.(prog_comp_env); genv_dropm := generate_dropm p |}.
+
+(** ** Evaluation of expressions *)
+
+Section EXPR.
+  
+Fixpoint eval_pexpr (e: sv_map) (pe: pexpr) : res sval :=
+  match pe with
+  | Eunit => OK (sv_scalar (Vint Int.zero))
+  | Econst_int i ty => OK (sv_scalar (Vint i))
+  | Econst_float f ty => OK (sv_scalar (Vfloat f))
+  | Econst_single f ty => OK (sv_scalar (Vsingle f))
+  | Econst_long i ty => OK (sv_scalar (Vlong i))
+  | Eunop op a t =>
+      do v1 <- eval_pexpr e a;
+      match v1 with
+      | sv_scalar v2 =>
+          match sem_unary_operation op v2 t with
+          | Some v3 =>
+              OK (sv_scalar v3)
+          | None =>
+              Error nil
+          end
+      | _ => Error nil
+      end
+  | Ebinop op a1 a2 t =>
+      do v1 <- eval_pexpr e a1;
+      do v2 <- eval_pexpr e a2;
+      match v1, v2 with
+      | sv_scalar v1', sv_scalar v2' =>
+          match sem_binary_operation_rust op v1' (typeof_pexpr a1) v2' (typeof_pexpr a2) with
+          | Some v =>
+              OK (sv_scalar v)
+          | None =>
+              Error nil
+          end
+      | _, _ => Error nil
+      end
+  | Eplace p ty =>
+      do ph <- get_owner_path_sv_map p e;
+      get_owner_sval_map ph e
+  | Ecktag p fid =>
+      do ph <- get_owner_path_sv_map p e;
+      do v <- get_owner_sval_map ph e;
+      match v with
+      | sv_enum _ fid1 _ =>
+          OK (sv_scalar (Val.of_bool (ident_eq fid fid1)))
+      | _ => Error nil
+      end
+  | Eref _ _ p _ =>
+      OK (sv_ref p)
+  | _ => Error nil
+  end.
+      
+Definition eval_expr (e: sv_map) (a: expr) : res (sval * sv_map) :=
+  match a with
+  | Emoveplace p _ =>
+      do v <- get_owner_sval_map p e;
+      do e1 <- clear_sval_map p e;
+      OK (v, e1)
+  | Epure pe =>
+      do v <- eval_pexpr e pe;
+      OK (v, e)
+  end.
+
+Fixpoint eval_exprlist (m: sv_map) (al: list expr) (tyl: typelist) : res (list sval * sv_map) :=
+  match al, tyl with
+  | nil, Tnil => OK (nil, m)
+  | a :: al1, Tcons ty tyl1 =>
+      do (v1, m1) <- eval_expr m a;
+      do v1' <- sem_cast v1 (typeof a) ty;
+      do (vl, m2) <- eval_exprlist m1 al1 tyl1;
+      OK (v1' :: vl, m2)
+  | _, _ => Error nil
+  end.
+
+End EXPR.
+
+(** ** Program states *)
+
+Inductive cont : Type :=
+| Kstop: cont
+| Kseq: statement -> cont -> cont
+| Kloop: statement -> cont -> cont
+| Kcall: place -> function -> list path -> list ident -> sv_map -> cont -> cont
+.
+
+
+(* Return from dropstate, dropplace and dropinsert is UB *)
+Fixpoint call_cont (k: cont) : option cont :=
+  match k with
+  | Kseq _ k => call_cont k
+  | Kloop _ k => call_cont k
+  | _ => Some k
+  end.
+
+
+Definition is_call_cont (k: cont) : Prop :=
+  match k with
+  | Kstop => True
+  | Kcall _ _ _ _ _ _ => True
+  | _ => False
+  end.
+
+Inductive state: Type :=
+| State
+    (f: function)
+    (s: statement)
+    (k: cont)
+    (names: list ident)         (* used to record the new idents for the in-out parameters *)
+    (e: sv_map): state
+| Callstate
+    (fun_id: ident)
+    (args: list sval)
+    (in_params: list sval) 
+    (k: cont): state
+| Returnstate
+    (res: sval)
+    (out_params: list sval)
+    (k: cont): state.
+
+
+(* Initialize of function *)
+
+(* Copy from memory *)
+
+Fixpoint find_max_pos (l: list positive) : positive :=
+  match l with
+  |nil => 1
+  |hd::tl => Pos.max hd (find_max_pos tl)
+  end.
+
+Fixpoint npos (n: nat) (p: positive) : list positive :=
+  match n with
+  | O => nil
+  | S n' =>
+      p :: (npos n' (Pos.succ p))
+  end.
+
+Fixpoint bind_params (m: sv_map) (l: list ident) (vl: list sval) : res sv_map :=
+  match l, vl with
+  | nil, nil => OK m
+  | id :: l1, v :: vl1 =>
+      do m1 <- set_sval_map (id, nil) v m;
+      bind_params m1 l1 vl1
+  | _, _ => Error nil
+  end.
+      
+
+Definition function_entry (f: function) (args: list sval) (in_params: list sval) : res (list ident * sv_map) :=
+  let names := field_idents (fn_params f ++ fn_vars f) in
+  let fresh_var := Pos.succ (find_max_pos names) in
+  let fresh_vars := npos (length in_params) fresh_var in
+  (* Substitute the old name in args and in_params with the fresh names *)
+  let fresh_paths : list path := map (fun id => (id, nil)) fresh_vars in
+  do args1 <- mmap (recover_sval_ref_paths fresh_paths) args;
+  do in_params1 <- mmap (recover_sval_ref_paths fresh_paths) in_params;
+  (* set the value to the map *)
+  do m1 <- bind_params (PTree.empty sval) (field_idents (fn_params f)) args1;
+  do m2 <- bind_params m1 fresh_vars in_params1;
+  do m3 <- bind_params m2 (field_idents (fn_vars f)) (repeat sv_bot (length (fn_vars f)));
+  OK (fresh_vars, m3).
+
+Section SMALLSTEP.
+
+Variable ge: genv.
+
+Inductive step : state -> trace -> state -> Prop :=
+| step_assign: forall f e (p: place) m1 m2 m3 ph v v1 ns k
+    (EVALP: get_owner_path_sv_map p m1 = OK ph)
+    (EVALE: eval_expr m1 e = OK (v, m2))
+    (CAST: sem_cast v (typeof e) (typeof_place p) = OK v1)
+    (ASS: set_sval_map ph v1 m2 = OK m3),
+    step (State f (Sassign p e) k ns m1) E0 (State f Sskip k ns m3)
+| step_assign_variant: forall f e (p: place) k m1 m2 m3 v v1 co fid enum_id orgs ph fty ns
+    (EVALP: get_owner_path_sv_map p m1 = OK ph)
+    (EVALE: eval_expr m1 e = OK (v, m2))
+    (* necessary for clightgen simulation *)
+    (TYP: typeof_place p = Tvariant orgs enum_id)
+    (CO: ge.(genv_cenv) ! enum_id = Some co)
+    (FTY: field_type fid co.(co_members) = OK fty)
+    (CAST: sem_cast v (typeof e) fty = OK v1)
+    (ASS: set_sval_map ph (sv_enum enum_id fid v1) m2 = OK m3),
+    step (State f (Sassign_variant p enum_id fid e) k ns m1) E0 (State f Sskip k ns m3)
+| step_box: forall f e (p: place) k ty m1 m2 m3 v v1 ph ns
+    (EVALP: get_owner_path_sv_map p m1 = OK ph)
+    (EVALE: eval_expr m1 e = OK (v, m2))
+    (TYP: typeof_place p = Tbox ty)
+    (CAST: sem_cast v (typeof e) ty = OK v1)
+    (ASS: set_sval_map ph (sv_box v1) m2 = OK m3),
+    step (State f (Sbox p e) k ns m1) E0 (State f Sskip k ns m3)
+(** bigl-step drop semantics: just like a move operation *)
+| step_drop: forall m1 m2 k f (p: place) ph ns
+    (EVALP: get_owner_path_sv_map p m1 = OK ph)
+    (DROP: clear_sval_map ph m1 = OK m2),
+    step (State f (Sdrop p) k ns m1) E0 (State f Sskip k ns m2)
+| step_storagelive: forall f k ns m id,
+    step (State f (Sstoragelive id) k ns m) E0 (State f Sskip k ns m)
+| step_storagedead: forall f k ns m id,
+    step (State f (Sstoragedead id) k ns m) E0 (State f Sskip k ns m)
+| step_call: forall f ty al k tyargs fd cconv tyres p orgs org_rels fun_id m1 m2 args args1 out_params ns phl
+    (CASE: classify_fun ty = fun_case_f tyargs tyres cconv)
+    (FINDF: ge.(genv_defmap) ! fun_id = Some (Gfun fd))
+    (TYF: type_of_fundef fd = Tfunction orgs org_rels tyargs tyres cconv)
+    (EVAL: eval_exprlist m1 al tyargs = OK (args, m2))
+    (NOT_DROP: function_not_drop_glue fd)
+    (* Collect the footprint that is passed via reference *)
+    (REF_OUT: generate_output_parameters m2 args = OK (args1, out_params, phl)),
+    step (State f (Scall p (Eglobal fun_id ty) al) k ns m1) E0 (Callstate fun_id args1 out_params (Kcall p f phl ns m2 k))
+| step_internal_function: forall fun_id vargs in_params k m f ns
+    (FINDF: ge.(genv_defmap) ! fun_id = Some (Gfun (Internal f)))
+    (NORMAL: f.(fn_drop_glue) = None)
+    (ENTRY: function_entry f vargs in_params = OK (ns, m)),
+    step (Callstate fun_id vargs in_params k) E0 (State f f.(fn_body) k ns m)
+
+(** We do not support axiomatic external call *)
+(* | step_external_function: forall vf vargs k m m' cc ty typs ef v t orgs org_rels *)
+(*     (FIND: Genv.find_funct ge vf = Some (External orgs org_rels ef typs ty cc)) *)
+(*     (NORMAL: ef <> EF_malloc /\ ef <> EF_free), *)
+(*     external_call ef ge vargs m t v m' -> *)
+(*     step (Callstate vf vargs k m) t (Returnstate v k m') *)
+   
+(** Return cases *)
+(* | step_return_0: forall e lb m1 m2 f k, *)
+(*     (forall id b t, e ! id = Some (b, t) -> complete_type ge t = true) -> *)
+(*     blocks_of_env ge e = lb -> *)
+(*     (* drop the stack blocks *) *)
+(*     Mem.free_list m1 lb = Some m2 -> *)
+(*     (* return unit or Vundef? *) *)
+(*     step (State f (Sreturn None) k e m1) E0 (Returnstate Vundef (call_cont k) m2) *)
+| step_return_1: forall p v v1 m1 f k ck ns
+    (CONT: call_cont k = Some ck)
+    (EVAL: eval_pexpr m1 (Eplace p (typeof_place p)) = OK v)
+    (CAST: sem_cast v (typeof_place p) f.(fn_return) = OK v1),
+    (** TODO: Rename the external footprint to match the use of the names passed
+    in this function *)
+    (** TODO: recover_sval_ref_paths may be a general definition, see
+    how to use it to define general name substitution for sval? *)
+    step (State f (Sreturn p) k ns m1) E0 (Returnstate v1 nil ck)
+(* no return statement but reach the end of the function *)
+(* | step_skip_call: forall e lb m1 m2 f k, *)
+(*     is_call_cont k -> *)
+(*     (forall id b t, e ! id = Some (b, t) -> complete_type ge t = true) -> *)
+(*     blocks_of_env ge e = lb -> *)
+(*     Mem.free_list m1 lb = Some m2 -> *)
+(*     step (State f Sskip k e m1) E0 (Returnstate Vundef (call_cont k) m2) *)
+         
+| step_returnstate: forall (p: place) v v1 m1 m2 m3 f k out_params phl ph ns
+    (* We need to first putback the ref-passed location and the do the
+    assignment because p may locate in those ref-passed locations *)
+    (PUTBACK: receive_return_sval m1 phl v out_params = OK (v1, m2))
+    (EVALP: get_owner_path_sv_map p m1 = OK ph)
+    (CASTED: val_casted v1 (typeof_place p))
+    (ASS: set_sval_map ph v1 m2 = OK m3),
+    step (Returnstate v out_params (Kcall p f phl ns m1 k)) E0 (State f Sskip k ns m2)
+
+(* Control flow statements *)
+| step_seq:  forall f s1 s2 k e m,
+    step (State f (Ssequence s1 s2) k e m)
+      E0 (State f s1 (Kseq s2 k) e m)
+| step_skip_seq: forall f s k e m,
+    step (State f Sskip (Kseq s k) e m)
+      E0 (State f s k e m)
+| step_continue_seq: forall f s k e m,
+    step (State f Scontinue (Kseq s k) e m)
+      E0 (State f Scontinue k e m)
+| step_break_seq: forall f s k e m,
+    step (State f Sbreak (Kseq s k) e m)
+      E0 (State f Sbreak k e m)
+| step_ifthenelse:  forall f a s1 s2 k e m v1 b
+    (* there is no receiver for the moved place, so it must be None *)
+    (EVAL: eval_pexpr m a = OK (sv_scalar v1)),
+    bool_val v1 (typeof a) = Some b ->
+    step (State f (Sifthenelse (Epure a) s1 s2) k e m)
+      E0 (State f (if b then s1 else s2) k e m)
+| step_loop: forall f s k e m,
+    step (State f (Sloop s) k e m)
+      E0 (State f s (Kloop s k) e m)
+| step_skip_or_continue_loop:  forall f s k e m x,
+    x = Sskip \/ x = Scontinue ->
+    step (State f x (Kloop s k) e m)
+      E0 (State f s (Kloop s k) e m)
+| step_break_loop:  forall f s k e m,
+    step (State f Sbreak (Kloop s k) e m)
+      E0 (State f Sskip k e m)
+.
+
+(** Language interfaces for the RustIR specification *)
+
+Record rust_spec_query :=
+  rspec_q {
+    rspec_fid: ident;
+    rspec_sg: rust_signature;
+    rspec_args: list sval;
+    rspec_in_params: list sval;
+  }.
+
+Record rust_spec_reply :=
+  rspec_r {
+    rspec_retval: sval;
+    rspec_out_params: list sval;
+  }.
+
+Definition li_rs_spec : language_interface :=
+  {|
+    query := rust_spec_query;
+    reply := rust_spec_reply;
+    entry _ := Vundef;
+  |}.
+
+
+(** Open semantics *)
+
+Inductive initial_state: (query li_rs_spec) -> state -> Prop :=
+| initial_state_intro: forall f targs tres tcc vargs orgs org_rels fun_id in_params
+    (FINDF: ge.(genv_defmap) ! fun_id = Some (Gfun (Internal f)))
+    (TYF: type_of_function f = Tfunction orgs org_rels targs tres tcc)
+    (* This function must not be drop glue *)
+    (NOTDROP: f.(fn_drop_glue) = None)
+    (* how to use it? *)
+    (CAST: val_casted_list vargs targs),
+    (* Mem.sup_include (Genv.genv_sup ge) (Mem.support m) -> *)
+    initial_state (rspec_q fun_id (mksignature orgs org_rels (type_list_of_typelist targs) tres tcc ge) vargs in_params)
+      (Callstate fun_id vargs in_params Kstop).
+
+
+Inductive at_external: state -> (query li_rs_spec) -> Prop :=
+| at_external_intro: forall fun_id name args k targs tres cconv orgs org_rels in_params
+    (FINDF: ge.(genv_defmap) ! fun_id = Some (Gfun (External orgs org_rels (EF_external name (signature_of_type targs tres cconv)) targs tres cconv))),
+    at_external (Callstate fun_id args in_params k) (rspec_q fun_id (mksignature orgs org_rels (type_list_of_typelist targs) tres cconv ge) args in_params).
+
+Inductive after_external: state -> (reply li_rs_spec) -> state -> Prop:=
+| after_external_intro: forall fun_id args k in_params out_params v,
+    after_external
+      (Callstate fun_id args in_params k)
+      (rspec_r v out_params)
+      (Returnstate v out_params k).
+
+Inductive final_state: state -> (reply li_rs_spec) -> Prop:=
+| final_state_intro: forall v out_params,
+    final_state (Returnstate v out_params Kstop) (rspec_r v out_params).
+
+End SMALLSTEP.
+
+End SEMANTICS.
+
+Definition semantics (p: program) :=
+  Semantics_gen step initial_state at_external (fun _ => after_external) (fun _ => final_state) globalenv p.
+
