Makefile
@@ -175,7 +175,7 @@ RUSTFRONTEND=Rusttypes.v Rustsyntax.v Rustlight.v RustIR.v\
   MoveChecking.v MoveCheckingFootprint1.v \
   Clightgen.v Clightgenspec.v Clightgenproof.v\
   RustOp.v Rusttyping.v\
-  StkBorPermission.v RustIRbor.v\
+  StkBorPermission.v RustIRbor.v RustIRspec.v\
   BorrowCheckDomain.v ReplaceOrigins.v BorrowCheckPolonius.v\
   RegionLiveness.v BorrowCheck.v BorrowCheckInv.v BorrowCheckSound.v\
   Listmisc.v\
